commit

AP/AP/DisjA.lean
@@ -3,7 +3,7 @@ import AP.AP.FSP
 namespace AP
 
 def State.aWinsDisj (s : State) (fsp : FSP) (st : Strat) : Prop :=
-  ∀ n, ∃ s₁, sys.simulate st.f s n = (s₁, 0) ∧ fsp.hasLe n s₁.aPos
+  ∀ n, ∃ s₁, sys.simulate st.f s n = (s₁, 0) ∧ ¬fsp.hasLe n s₁.aPos
 
 def State.aHwsDisj (s : State) (fsp : FSP) : Prop :=
   ∃ (a : AStrat), a.WF ∧ ∀ (d : DStrat), d.WF → s.aWinsDisj fsp ⟨a, d⟩
@@ -42,3 +42,71 @@ theorem DState.tr_of_aHwsDisj {s s' p fsp} [hs : DState s] (h₁ : s.aHwsDisj fs
   have hs' := sys.wf_of_tr h₂
   apply simulate_set_d_eq_of_length_hist_lt ⟨_, h₂⟩
   exact State.length_hist_lt_of_tr h₂
+
+theorem State.aWinsDisj_iff {s : State} {fsp} {st : Strat} :
+s.aWinsDisj fsp st ↔ s.aWins st ∧ ∀ n, ¬fsp.hasLe n (sys.simulate st.f s n).1.aPos := by
+  constructor
+  · intro h
+    constructor
+    · intro n
+      specialize h n
+      aesop
+    intro n
+    specialize h n
+    aesop
+  rintro ⟨h₁, h₂⟩
+  intro n
+  simp [Prod.ext_iff]
+  specialize h₁ n
+  aesop
+
+-- #check 0 #exit
+
+theorem State.aHwsDisj_insert {s fsp p} [hs : sys.WF s]
+(h₁ : s.aHwsDisj fsp) : ∃ n, s.aHwsDisj (fsp.insert n p) := by
+  unfold aHwsDisj aWinsDisj at h₁ ⊢
+  by_contra! h₃
+  replace h₃ : ∀ (a : AStrat) [a.WF] n, ∃ (d : DStrat), d.WF ∧ ∃ k, n ≤ k ∧
+    ∀ s₁ r, sys.simulate (Strat.f ⟨a, d⟩) s k = ⟨s₁, r⟩ →
+    r ≠ 0 ∨ ¬(fsp.insert n p).hasLe k s₁.aPos
+  · intro a Ha n
+    sorry
+  sorry
+
+-- #check 0 #exit
+
+theorem State.aHwsDosj_insertSet_of_le {s : State} {fsp : FSP} {m n ps}
+(h₁ : s.aHwsDisj (fsp.insertSet m ps)) (h₂ : m ≤ n) : s.aHwsDisj (fsp.insertSet n ps) := by
+  obtain ⟨a, Ha, h₁⟩ := h₁
+  use a, Ha
+  intro d Hd
+  specialize h₁ d Hd
+  rw [aWinsDisj_iff] at h₁ ⊢
+  rcases h₁ with ⟨h₁, h₃⟩
+  use h₁; clear h₁
+  intro k
+  specialize h₃ k
+  generalize (sys.simulate (Strat.f ⟨a, d⟩) s k).1 = s₁ at h₃ ⊢
+  contrapose! h₃
+  exact fsp.hasLe_insertSet_of_le_and_le h₃ h₂
+
+theorem State.aHwsDosj_insert_of_le {s : State} {fsp : FSP} {m n p}
+(h₁ : s.aHwsDisj (fsp.insert m p)) (h₂ : m ≤ n) : s.aHwsDisj (fsp.insert n p) :=
+  aHwsDosj_insertSet_of_le h₁ h₂
+
+theorem State.aHwsDisj_insertSet' {s fsp}  {ps : Set' PointZ} [hs : sys.WF s]
+(h₁ : s.aHwsDisj fsp) : ∃ n, s.aHwsDisj (fsp.insertSet n ps.toSet) := by
+  induction ps using Set'.ind; simpa; clear h₁
+  nm ps p hp ih
+  obtain ⟨n, ih⟩ := ih
+  obtain ⟨m, h₂⟩ := s.aHwsDisj_insert ih (p := p)
+  use max n m; simp
+  rw [fsp.insertSet_set_insert]
+  apply aHwsDosj_insert_of_le _ # Nat.le_max_right n m
+  rw [fsp.insertSet_insert_comm] at h₂ ⊢
+  exact aHwsDosj_insertSet_of_le h₂ # Nat.le_max_left n m
+
+theorem State.aHwsDisj_insertSet_of_finite {s fsp ps} [hs : sys.WF s]
+(h₁ : s.aHwsDisj fsp) (h₂ : ps.Finite) : ∃ n, s.aHwsDisj (fsp.insertSet n ps) := by
+  have h₃ := s.aHwsDisj_insertSet' (ps := Set'.ofSet ps) h₁
+  rwa [Set'.toSet_ofSet h₂] at h₃
