AP/AP/FSP.lean
@@ -2,12 +2,13 @@ import AP.AP.MkFold
 
 namespace AP
 
+@[ext]
 structure FSP : Type where
   get : ℕ → Set PointZ
 
 namespace FSP
 
-variable {a b c : FSP}
+variable {fsp a b c : FSP}
 
 instance : EmptyCollection FSP := ⟨⟨λ _ => ∅⟩⟩
 theorem empty_def : (∅ : FSP) = ⟨λ _ => ∅⟩ := rfl
@@ -21,17 +22,17 @@ theorem union_def : a ∪ b = ⟨λ i => a.get i ∪ b.get i⟩ := rfl
 instance : Inter FSP := ⟨λ a b => ⟨λ i => a.get i ∩ b.get i⟩⟩
 theorem inter_def : a ∩ b = ⟨λ i => a.get i ∩ b.get i⟩ := rfl
 
-def next (a : FSP) : FSP := .mk # λ i =>
-  match i with
+def next (a : FSP) : FSP where
+  get i := match i with
   | 0 => a.get 0 ∪ a.get 1
   | n + 1 => a.get # n + 2
 
 def hasLe (a : FSP) (n : ℕ) (p : PointZ) : Prop :=
-  ∀ k ≤ n, p ∉ a.get k
+  ∃ k ≤ n, p ∈ a.get k
   
 @[simp]
 theorem hasLe_next {n p} : a.next.hasLe n p ↔ a.hasLe (n + 1) p := by
-  dsimp [next, hasLe]
+  rw [←not_iff_not]; dsimp [next, hasLe]; push_neg
   constructor <;> intro h k hk
   · specialize h (k - 1) # Nat.sub_le_of_le_add hk
     iterate 2 cases k; simp at h; simp [h]; nm k
@@ -39,3 +40,77 @@ theorem hasLe_next {n p} : a.next.hasLe n p ↔ a.hasLe (n + 1) p := by
   · have h₁ := h k (by linarith)
     have h₂ := h (k + 1) (by simpa)
     cases k <;> simp_all
+
+def insertSet (fsp : FSP) (n : ℕ) (ps : Set PointZ) : FSP where
+  get i := if i = n then ps ∪ fsp.get i else fsp.get i
+
+protected def insert (fsp : FSP) (n : ℕ) (p : PointZ) : FSP :=
+  fsp.insertSet n {p}
+
+theorem hasLe_insertSet_eq_of_lt {n k ps} (h : k < n) :
+(fsp.insertSet n ps).hasLe k = fsp.hasLe k := by
+  ext p; rw [←not_iff_not]; dsimp [hasLe, insertSet]; push_neg
+  apply forall_congr'
+  intro i
+  split_ifs with h₁
+  · subst h₁
+    rw [←not_le] at h
+    simp [h]
+  simp
+
+theorem hasLe_insert_eq_of_lt {n k p} (h : k < n) :
+(fsp.insert n p).hasLe k = fsp.hasLe k := hasLe_insertSet_eq_of_lt h
+
+@[simp]
+theorem insertSet_empty {n} : fsp.insertSet n ∅ = fsp := by
+  simp [insertSet]
+
+theorem insertSet_insert {n p ps} :
+(fsp.insertSet n ps).insert n p = fsp.insertSet n (insert p ps) := by
+  unfold FSP.insert insertSet; aesop
+
+theorem insertSet_set_insert {n p ps} :
+fsp.insertSet n (insert p ps) = (fsp.insertSet n ps).insert n p :=
+  insertSet_insert.symm
+
+@[simp]
+theorem get_insertSet_of_eq {n ps} : (fsp.insertSet n ps).get n = ps ∪ fsp.get n := by
+  simp [insertSet]
+
+@[simp]
+theorem get_insert_of_eq {n p} : (fsp.insert n p).get n = insert p (fsp.get n) := by
+  simp [FSP.insert]
+
+theorem hasLe_insertSet_of_le {m n k ps p} (h₁ : (fsp.insertSet m ps).hasLe k p)
+(h₂ : m ≤ k) (h₃ : n ≤ k) : (fsp.insertSet n ps).hasLe k p := by
+  obtain ⟨r, hr, h₁⟩ := h₁
+  by_cases hp : p ∈ ps
+  · use n, h₃; simp [hp]
+  use r, hr
+  simp [insertSet] at h₁ ⊢
+  aesop
+
+theorem insertSet_comm {n m ps₁ ps₂} : (fsp.insertSet n ps₁).insertSet m ps₂ =
+(fsp.insertSet m ps₂).insertSet n ps₁ := by
+  unfold insertSet; aesop
+
+theorem insert_comm {n m p₁ p₂} : (fsp.insert n p₁).insert m p₂ =
+(fsp.insert m p₂).insert n p₁ := insertSet_comm
+
+theorem insertSet_insert_comm {n m ps₁ p₂} : (fsp.insertSet n ps₁).insert m p₂ =
+(fsp.insert m p₂).insertSet n ps₁ := insertSet_comm
+
+theorem insert_insertSet_comm {n m p₁ ps₂} : (fsp.insert n p₁).insertSet m ps₂ =
+(fsp.insertSet m ps₂).insert n p₁ := insertSet_comm
+
+theorem hasLe_insertSet_of_hasLe {n k ps p} (h₁ : fsp.hasLe k p) :
+(fsp.insertSet n ps).hasLe k p := by
+  dsimp [insertSet, hasLe] at h₁ ⊢; aesop
+
+theorem hasLe_insertSet_of_le_and_le {m n k ps p} (h₁ : (fsp.insertSet n ps).hasLe k p)
+(h₂ : m ≤ n) : (fsp.insertSet m ps).hasLe k p := by
+  by_cases h₃ : n ≤ k
+  · exact hasLe_insertSet_of_le h₁ h₃ # h₂.trans h₃
+  push_neg at h₃
+  rw [hasLe_insertSet_eq_of_lt h₃] at h₁
+  exact hasLe_insertSet_of_hasLe h₁
